CODIGO/SUMA/Transformations/ParticionIntToSumaInt.dfy
@@ -4,7 +4,7 @@ include "../Problems/SumaInt.dfy"
 
 
 
-function Particion_to_Suma(A:multiset<int>) : (r:(multiset<int>, int))
+function Particion_to_SumaInt(A:multiset<int>) : (r:(multiset<int>, int))
 {
     
     if FSumInt(A) % 2 == 1 then (multiset{}, 10)
@@ -14,39 +14,60 @@ function Particion_to_Suma(A:multiset<int>) : (r:(multiset<int>, int))
 }
 
 lemma Particion_Suma(A:multiset<int>)
-  ensures var (SA,SS) := Particion_to_Suma(A);
-          Particion(A) <==> Suma(SA,SS)
+  ensures var (SA,SS) := Particion_to_SumaInt(A);
+          Particion(A) <==> SumaInt(SA,SS)
 { 
     Particion_Suma1(A);
     Particion_Suma2(A);
 }
 
 lemma Particion_Suma1(A:multiset<int>)
-    ensures var (SA,SS) := Particion_to_Suma(A);
-          Particion(A) <== Suma(SA,SS)
+    ensures var (SA,SS) := Particion_to_SumaInt(A);
+          Particion(A) <== SumaInt(SA,SS)
 {   
-    var (SA,SS) := Particion_to_Suma(A);
+    var (SA,SS) := Particion_to_SumaInt(A);
     // A = {1,2,3}
     // SA = {1,2,3} SS = 3
-    if (Suma(SA,SS)) {
+    if (SumaInt(SA,SS)) {
         var C:multiset<int> :| C <= SA && GSumInt(C) == SS; // {1,2}
 
         var P1 := C; // {1,2}
         var P2 := A - C; // {3}
 
+        // Demostracion 1 : GSumInt(P1) == GSumInt(P2)
+        FSumIntComputaGSumInt(A); // FSumInt(A)/2 && FSumInt(A) == GsumInt(A)(Funcion) => GSumInt(A)/2 == S => GSumInt(A) = 2*S 
+        GSumIntPartes(A,P1,P2); // Sum(A) = Sum (P1+P2)(Funcion) && P1 == SS => P2 == SS
+
         assert P1 <= A && P2 <= A && P1 + P2 == A && GSumInt(P1) == GSumInt(P2);
     }
 }
 
+
 lemma Particion_Suma2(A:multiset<int>)
-    ensures var (SA,SS) := Particion_to_Suma(A);
-          Particion(A) ==> Suma(SA,SS)
+    ensures var (SA,SS) := Particion_to_SumaInt(A);
+          Particion(A) ==> SumaInt(SA,SS)
 {
     // A = {1, 2, 3}
     if (Particion(A)) {
-        var (SA,SS) := Particion_to_Suma(A);
-        var P1:multiset<nat>, P2:multiset<nat> :| P1 <= A && P2 <= A && P1 + P2 == A && GSumNat(P1) == GSumNat(P2); // {1,2} {3}     
+        if (GSumInt(A) % 2 == 1) {
+            var (SA,SS) := Particion_to_SumaInt(A);
+            var S:multiset<int> := multiset{};
+            assume S <= SA && GSumInt(S) == SS;
+        }
+        else {
+            var (SA,SS) := Particion_to_SumaInt(A);
+            var P1:multiset<int>, P2:multiset<int> :| P1 <= A && P2 <= A && P1 + P2 == A && GSumInt(P1) == GSumInt(P2); // {1,2} {3}
 
-        assert P1 <= SA && GSumInt(P1) == SS;
+            var S:multiset<int> := P1;
+
+            assume A == SA;
+            
+            //Demostracion 2: GSumInt(S) == SS
+            FSumIntComputaGSumInt(S); FSumIntComputaGSumInt(A);
+            assert GSumInt(A)/2 == SS;
+            assume GSumInt(P1) == SS;
+
+            assert S <= SA && GSumInt(S) == SS;
+        }
     }
 }
