CODIGO/SUMA/Problems/Intercalar.dfy
@@ -11,10 +11,11 @@ ghost predicate Intercalar(E:seq<nat>)
 {
   if (|E| == 0) then true
   else
-   var elements:= multiset(E);
+   var elements:multiset<nat> := multiset(E);
    exists E1,E2 :: 
-     E[0] in E1 && E1 <= elements //E1 positive elements
-     && E2 <= elements               //E2 negative elements
+     E[0] in E1 
+     && E1 <= elements     //E1 positive elements
+     && E2 <= elements                //E2 negative elements
      && E1 + E2 == elements
-     && GSumInt(E1) - GSumInt(E2) == 0
+     && GSumNat(E1) - GSumNat(E2) == 0
 }
